agreeonread_w_r

semantics/proofs_w.v
@@ -14,6 +14,9 @@ Inductive all_diff_in_fww: nvmem -> vmem -> command -> nvmem -> Prop :=
 ( forall(l: loc ), ((getmap N1) l <> (getmap N1c) l) -> (l \in getfstwt W))
 -> all_diff_in_fww N1 V1 c1 N1c.
 
+ Lemma add_skip_ins_w {N1 V l N2}: all_diff_in_fww N1 V (Ins l) N2 ->
+                                 all_diff_in_fww N1 V (l;; skip) N2.
+   Admitted.
     Lemma agreeonread_ins_w_r: forall{N Nend N2: nvmem} {V Vend: vmem}
                         {l: instruction} {crem c1: command}
                    {O : obseq} {W: the_write_stuff},
@@ -71,7 +74,30 @@ Inductive all_diff_in_fww: nvmem -> vmem -> command -> nvmem -> Prop :=
             ( forall(z: loc), z \in (getrd W) -> (*z was read immediately cuz trace is only 1
                                 thing long*)
                    (getmap N2) z = (getmap N) z). (*since z isnt in FW of trace from Ins l to skip*)
- Admitted.
+   intros. move: H H0 H1 => Hdiff Hcc Hr. dependent induction c.
+   apply add_skip_ins_w in Hdiff.
+   eapply agreeonread_ins_w_r; try apply Hdiff; try apply Hcc; try assumption.
+   inversion Hcc; subst; try( rewrite in_nil in Hr; discriminate Hr).
+   eapply agreeonread_ins_w_r; try apply Hdiff; try apply H10; try assumption.
+   inversion Hdiff; subst.
+   apply/eqP /negPn/ negP. intros contra. move/eqP: contra => contra.
+   apply not_eq_sym in contra. apply (H0 z) in contra.
+      destruct (O0 == [::]) eqn: Hbool; move/eqP : Hbool => Heq; subst.
+      - 
+        move: (empty_trace_cs1 T) => [ [one two] three four].
+        subst. discriminate contra.
+      - 
+        move: (single_step_alls_rev T Heq) =>
+        [Cmid [W1 [Wrest [O1 [Hcceval [Hsubseq Hw] ] ] ] ] ].
+        move: (cceval_agr Hcceval Hcc) => Hww.
+        rewrite Hw in contra.
+        unfold append_write in contra. simpl in contra. rewrite Hww in contra. rewrite - Hww in Hr.
+        move: (r_means_negfw Hcceval Hr) => Hfw.
+        rewrite mem_cat in contra.
+        move/ orP : contra. => [con1 | con2].
+        rewrite mem_filter in con1. move/andP: con1 => [con11 con12]. move/ negP: con11. apply. by rewrite - Hww.
+        move/ negP: Hfw. by apply.
+    Qed.
 
  (*bassically same as proving proofs_new lemma*)
  Lemma agreeonread_w_l: forall{N Nend N2: nvmem} {V Vend: vmem}
@@ -161,9 +187,6 @@ move: (agreeonread_ins_w_r Hdiff Hcceval1) => agr.
           by apply Hneq.
 Qed.*)
 
- Lemma add_skip_ins_w {N1 V l N2}: all_diff_in_fww N1 V (Ins l) N2 ->
-                                 all_diff_in_fww N1 V (l;; skip) N2.
-   Admitted.
 
 Lemma trace_converge_minus1w {N V N' Nmid Vmid Nmid'
                             O W} {l: instruction}:
